Rake: `ex_seq` lemma and proof stubs for `rem`.

Rake.lean
@@ -16,15 +16,9 @@ instance : CoeFun (DSeq d) fun _ => Nat → Nat := ⟨λs => s.val⟩
 -- within the rake at each step.
 instance : LE (DSeq d) where le a b := a.val.k ≤ b.val.k
 instance : IsTotal (DSeq d) (·≤·) := by
-  apply IsTotal.mk
-  intro a b
-  cases a; cases b
-  apply Nat.le_total
+  apply IsTotal.mk; intro a b; cases a; cases b; apply Nat.le_total
 instance : IsTrans (DSeq d) (·≤·) := by
-  apply IsTrans.mk
-  intro a b c
-  cases a; cases b; cases c
-  apply Nat.le_trans
+  apply IsTrans.mk; intro a b c; cases a; cases b; cases c; apply Nat.le_trans
 
 def dseq (k : Nat) (d : Nat) : DSeq d := ⟨ASeq.mk k d, rfl⟩
 
@@ -33,6 +27,12 @@ structure Rake where
   seqs : List (DSeq d)
   hsort : List.Sorted (·≤·) seqs
   hsize : seqs.length > 0
+
+def idr : Rake := { -- the identity rake (maps n -> n)
+  d := 1,
+  seqs := [dseq 0 1],
+  hsort := List.sorted_singleton _,
+  hsize := Nat.zero_lt_one }
 
 def Rake.term (r : Rake) (n : Nat) : Nat :=
   let q := r.seqs.length
@@ -49,21 +49,44 @@ def Rake.gte (r : Rake) (n : Nat) : Rake := {
   hsort := by apply List.sorted_mergeSort
   hsize := (by simp[List.length_mergeSort]; exact r.hsize)}
 
-def idr : Rake := { -- the identity rake (maps n -> n)
-  d := 1,
-  seqs := [dseq 0 1],
-  hsort := List.sorted_singleton _,
-  hsize := Nat.zero_lt_one }
+def Rake.rem (r : Rake) (n : Nat) : Rake := {
+  d := r.d
+  seqs := r.seqs.map (λ s => ⟨ASeq.gte s.val n, (by
+    have : s.val.d = r.d := s.property
+    symm at this
+    simp[this]
+    apply ASeq.gte_same_delta s.val n)⟩) |> List.mergeSort (·≤·)
+  hsort := by apply List.sorted_mergeSort
+  hsize := (by simp[List.length_mergeSort]; exact r.hsize)}
+
+-- rakemap --------------------------------------------------------------------
 
 structure RakeMap (prop: Nat → Prop) where
   rake : Rake
   hbij : ∀ n, prop n ↔ ∃ m, rake.term m = n
 
--- proof that idr.term provides a bijection from Nat → Nat
--- (it happens to be an identity map, but this is not necessary for proofs)
+/-- proof that idr.term provides a bijection from Nat → Nat
+ (it happens to be an identity map, but this is not necessary for proofs) -/
 def idrm : RakeMap (λ _ => True) := {
   rake := idr,
   hbij := by intro n; simp[Rake.term, idr]; unfold dseq; unfold term; simp }
+
+/-- proof that if a rakemap produces a term, it's because one of the sequences
+    it contains produces that term. -/
+lemma RakeMap.ex_seq (rm: RakeMap prop)
+  : (rm.rake.term m = n) → (∃seq ∈ rm.rake.seqs, ∃m₁, seq m₁ = n) := by
+  unfold Rake.term
+  intro hseq
+  set q := rm.rake.seqs.length
+  have : m%q < rm.rake.seqs.length := Nat.mod_lt _ rm.rake.hsize
+  let seq := rm.rake.seqs[m%q]
+  set m1 := m/rm.rake.seqs.length
+  use seq
+  apply And.intro
+  · exact List.get_mem rm.rake.seqs (m % q) this
+  · dsimp at hseq
+    dsimp[seq,q]
+    use m1
 
 section gte_lemmas
 
@@ -83,7 +106,29 @@ section gte_lemmas
 
 end gte_lemmas
 
-def RakeMap.gte_prop (prev : RakeMap prop) (p: Nat)
+section rem_lemmas
+
+  variable (rm: RakeMap prop) (p n: Nat)
+
+  lemma RakeMap.rem_drop -- rem drops multiples of p
+    : p∣n → ¬(∃m, (rm.rake.rem p).term m = n) := by
+    sorry
+
+  lemma RakeMap.rem_keep -- rem keeps non-multiples of p
+    : ¬(p∣n) ∧ (∃pm, rm.rake.term pm = n) → (∃m, (rm.rake.rem p).term m = n) := by
+    sorry
+
+  lemma RakeMap.rem_same -- rem introduces no new terms
+    : (∃pm, (rm.rake.rem p).term pm = n) → (∃pm, rm.rake.term pm = n) := by
+    sorry
+
+end rem_lemmas
+
+
+-- operations on RakeMap -------------------------------------------------------
+-- these proofs are exactly the same except for the proposition
+
+def RakeMap.gte (prev : RakeMap prop) (p: Nat)
   : RakeMap (λ n => prop n ∧ n ≥ p) :=
   let rake := prev.rake.gte p
   let proof := by
@@ -95,4 +140,18 @@ def RakeMap.gte_prop (prev : RakeMap prop) (p: Nat)
     have : n≥p ∧ hpm → hm := gte_keep prev p n
     have : hm → hpm := gte_same prev p n
     by_cases n<p; all_goals aesop
+  { rake := rake, hbij := proof }
+
+def RakeMap.rem (prev : RakeMap prop) (p: Nat)
+  : RakeMap (λ n => prop n ∧ ¬(p∣n)) :=
+  let rake := prev.rake.rem p
+  let proof := by
+    intro n; symm
+    let hm : Prop := (∃m, rake.term m = n)
+    let hpm : Prop := (∃pm, prev.rake.term pm = n )
+    have : prop n ↔ hpm := prev.hbij n
+    have : p∣n → ¬hm := rem_drop prev p n
+    have : ¬p∣n ∧ hpm → hm := rem_keep prev p n
+    have : hm → hpm := gte_same prev p n
+    by_cases p∣n; all_goals aesop
   { rake := rake, hbij := proof }
